IMP/My_Utils.thy
@@ -1,0 +1,92 @@
+theory My_Utils
+  imports Main
+begin
+
+(* TODO: move these utils into some better place *)
+
+
+definition "null = (\<lambda>_. undefined)"
+
+abbreviation "concat_map f xs \<equiv> concat (map f xs)"
+
+
+(* generate *)
+
+definition "generate f n \<equiv> map f [0..<n]"
+(* abbreviation "generate_len f xs \<equiv> generate f (length xs)" (* ? *) *)
+
+lemma generate_cong[fundef_cong]:
+  assumes "n = m" "\<And>i. i < m \<Longrightarrow> f i = g i"
+  shows "generate f n = generate g m"
+  using assms unfolding generate_def by simp
+
+lemma map_generate_comp: "map g (generate f n) = generate (g o f) n"
+  unfolding generate_def by simp
+
+lemma generate_snoc: "generate f (Suc n) = generate f n @ [f n]"
+  unfolding generate_def by auto
+
+lemma generate_length[simp]: "length (generate f n) = n"
+  unfolding generate_def by simp
+
+lemma generate_0_conv[iff]: "generate f n = [] \<longleftrightarrow> n = 0"
+  unfolding generate_def by simp
+
+(* like turning a classic for loop into a for-each loop *)
+lemma generate_nth_is_map[simp]: "generate (\<lambda>i. f (xs ! i)) (length xs) = map f xs"
+  unfolding generate_def by (simp add: map_equality_iff)
+
+
+(* sum_map *)
+
+abbreviation "sum_map f xs \<equiv> sum_list (map f xs)"
+
+lemma sum_map_concat: "sum_map f (concat xss) = sum_list (concat (map (map f) xss))"
+  using map_concat by metis
+
+lemma sum_map_mono:
+  fixes f g :: "'a \<Rightarrow> 'b :: {ordered_ab_semigroup_add, monoid_add}"
+  assumes "\<forall>x \<in> set xs. f x \<le> g x"
+  shows "sum_map f xs \<le> sum_map g xs"
+  using assms add_mono by (induction xs) auto
+
+
+(* max_list0 *)
+
+(* maximum of a list, but defined (as 0) for empty lists *)
+(* defined only on nat to keep things simple *)
+definition max_list0 :: "nat list \<Rightarrow> nat" where
+  "max_list0 xs \<equiv> fold max xs 0"
+
+lemma max_list0_cons:
+  shows "max_list0 (x # xs) = max x (max_list0 xs)"
+proof-
+  have "fold max (x # xs) z = max x (fold max xs z)" for xs :: "nat list" and x z
+    by (induction xs arbitrary: x z) simp_all
+  then show ?thesis unfolding max_list0_def by blast
+qed
+
+lemma max_list0_append: "max (max_list0 xs) (max_list0 ys) = max_list0 (xs @ ys)"
+proof (induction xs)
+  case Nil then show ?case using max_list0_def by simp
+  case (Cons a xs) then show ?case using max_list0_cons by simp
+qed
+
+
+(* max1 *)
+
+definition max1 :: "nat \<Rightarrow> nat" (\<open>(\<open>notation=\<open>postfix +\<close>\<close>_\<^sub>+)\<close> [1000] 999) where
+  "max1 \<equiv> max 1"
+
+lemma max1_idem[simp]: shows "(x\<^sub>+)\<^sub>+ = x\<^sub>+" unfolding max1_def by simp
+lemma max1_pos[simp]: "x\<^sub>+ \<noteq> 0" unfolding max1_def by simp
+lemma max1_pos_id[simp]: "x \<noteq> 0 \<Longrightarrow> x\<^sub>+ = x" unfolding max1_def by simp
+lemma max1_id_positive[iff]: "x\<^sub>+ = x \<longleftrightarrow> x \<noteq> 0" unfolding max1_def by linarith
+
+lemma max1_plus1[simp]: "x \<noteq> 0 \<Longrightarrow> (x + y)\<^sub>+ = x + y" by simp
+lemma max1_plus2[simp]: "y \<noteq> 0 \<Longrightarrow> (x + y)\<^sub>+ = x + y" by simp
+
+lemma max1_inc: "x\<^sub>+ \<ge> x" unfolding max1_def by simp
+
+
+end
